rupicola/io/RrHP.fst
@@ -21,17 +21,16 @@ noeq type intS = {
   // (proof of) compiled closed expression - where we pass in the type of ps (#_), the (proof of the) type of the compiled closed expression (#(compile_typ_arrow ...)), and ps
   // should exp_quotation also carry fs_event trace?
 type progS (i:intS) =
-  (ps:(get_Type i.ct -> bool) & exp_quotation #(i.ct ^-> qBool) empty (fun _ -> ps))
-  * 
-  (list fs_event * list event) // might need to change these to be dependent tuples
+  ps:(get_Type i.ct -> bool) 
+  & 
+  exp_quotation #(i.ct ^-> qBool) empty (fun _ -> ps)
 
 type ctxS (i:intS) = get_Type i.ct
 type wholeS = bool // CA: To be able to compile whole programs requires a proof that it can be compiled
 
 // linking involves taking a program and context, extracting the first part of the dependent pair (so the program i.ct -> bool) and applying it to the context
 let linkS (#i:intS) (ps:progS i) (cs:ctxS i) : wholeS =
-  let ((| fs_e, e |), (fs_e_tr, e_tr )) = ps in 
-  fs_e cs
+  (dfst ps) cs
 
 type behS_t = bool
 val behS : wholeS -> behS_t
@@ -48,7 +47,7 @@ val comp_int : intS -> intT
 //let comp_int i = { ct = type_quotation_to_typ i.qct }
 let comp_int i = { ct = i.ct }
 
-type progT (i:intT) = closed_exp * list event
+type progT (i:intT) = closed_exp
 
 // the typing makes sure that there are no pre post conditions - maybe...
 type ctxT (i:intT) = ct:value & typing empty ct i.ct
@@ -57,37 +56,31 @@ type wholeT = closed_exp
 
 let linkT (#i:intT) (pt:progT i) (ct:ctxT i) : wholeT =
   let (| e, h |) = ct in
-  let (e_pt, tr_pt) = pt in
-  let wt = EApp e_pt e in
+  let wt = EApp pt e in
   wt
 
 let compile_prog (#i:intS) (ps:progS i) : progT (comp_int i) =
-  let ((| fs_e, e |), (fs_tr, tr)) = ps in
-  ((compile_closed e), tr)
-  // needs to be fixed to be the list of events from quotation
+  compile_closed (dsnd ps)
 
 let rel_bools (fs_e:bool) (e:exp) : Type0 =
   (e == ETrue /\ fs_e == true) \/
   (e == EFalse /\ fs_e == false)
 
-let rel_traces (fs_tr:list fs_event) (tr:list event) : Type0 =
-  trace_related fs_tr tr
-
 type behT_t = bool -> Type0
-val behT : wt:wholeT -> tr:list event -> behT_t
-let behT wt tr = fun x -> // need to change this to rel_traces when we want to start looking at traces
+val behT : wt:wholeT -> behT_t
+let behT wt = fun x ->
 (** vvv To have an existential here one needs normalization **)
-  forall (e':closed_exp). steps wt e' tr /\ irred e' ==>
+  forall (e':closed_exp). steps wt e' /\ irred e' ==>
     rel_bools x e'
 
 val rel_behs : behS_t -> behT_t -> Type0
 let rel_behs (bs:behS_t) (bt:behT_t) =
   bt bs
 
-let lem_rel_beh (fs_e:wholeS) (fs_tr:list fs_event) (e:wholeT) (tr:list event)  
+let lem_rel_beh (fs_e:wholeS) (e:wholeT)  
   : Lemma
-  (requires qBool ⦂ ((fs_e, fs_tr), (e, tr)))
-  (ensures  (behS fs_e) `rel_behs` (behT e tr))
+  (requires qBool ⦂ (fs_e, e))
+  (ensures  (behS fs_e) `rel_behs` (behT e))
   = ()
 
 (** ** Proof of RrHP **)
@@ -100,48 +93,45 @@ let backtranslate_ctx (#i:intS) (ctxt:ctxT (comp_int i)) : ctxS i =
 
 val lem_bt_ctx i ct : Lemma (
   let (| e, h |) = ct in
-    (comp_int i).ct ∋ ((backtranslate_ctx #i ct, []), (e, []))
+    (comp_int i).ct ∋ (backtranslate_ctx #i ct, e)
   )
 let lem_bt_ctx i ct =
   let (| e, h |) = ct in
   lem_value_is_closed e;
   lem_closed_is_no_fv e;
   assert (fv_in_env empty e);
-  lem_backtranslate empty e (comp_int i).ct h #[] #[];
-  equiv_closed_terms #[] #[] #(comp_int i).ct (backtranslate empty e (comp_int i).ct h empty_eval) e;
+  lem_backtranslate empty e (comp_int i).ct h;
+  equiv_closed_terms #(comp_int i).ct (backtranslate empty e (comp_int i).ct h empty_eval) e;
   // t : (bt e, e) and the fact that e is a value implies they are in the value relation (the statement of the lemma)
   ()
 
 (** This variant implies RrHP **)
 let rrhp_1 (#i:intS) =
   forall (ps:progS i).
-    forall ct. behS (linkS ps (backtranslate_ctx ct)) `rel_behs` behT (linkT (compile_prog ps) ct) (snd (compile_prog ps) @ [])
+    forall ct. behS (linkS ps (backtranslate_ctx ct)) `rel_behs` behT (linkT (compile_prog ps) ct)
 
 let proof_rrhp_1 i : Lemma (rrhp_1 #i) =
-  introduce forall ps ct. behS (linkS ps (backtranslate_ctx ct)) `rel_behs` behT (linkT (compile_prog ps) ct) (snd (compile_prog ps) @ []) with begin
+  introduce forall ps ct. behS (linkS ps (backtranslate_ctx ct)) `rel_behs` behT (linkT (compile_prog ps) ct) with begin
     let t : qType = i.ct in
     let pt : progT (comp_int i) = compile_prog ps in
-    let ((| fs_e_ps, e_ps |), (fs_tr, tr)) = ps in
-    let ws : wholeS = fs_e_ps (backtranslate_ctx ct) in
+    let ws : wholeS = (dfst ps) (backtranslate_ctx ct) in
     let (| e, h |) = ct in
-    let (e_pt, tr_pt) = pt in
-    let wt : exp = EApp e_pt e in
+    let wt : exp = EApp pt e in
     let wt : wholeT = wt in
-    compile_equiv #empty #fs_tr #tr e_ps;
-    let ps' = fs_e_ps in
-    compile_closed_equiv #(t ^-> qBool) #_  #fs_tr #tr e_ps;
-    assert ((t ^-> qBool) ⦂ ((ps', fs_tr), (e_pt, tr_pt)));
-    lemma_compile_closed_arrow_is_elam e_ps;
-    assert (ELam? e_pt /\ is_closed e_pt /\ irred e_pt);
-    eliminate forall (e':closed_exp). steps e_pt e' tr_pt ==> irred e' ==> (t ^-> qBool) ∋ ((ps', fs_tr), (e', tr_pt)) with e_pt;
-    assume ((t ^-> qBool) ∋ ((ps', fs_tr), (e_pt, tr_pt)));
-    eliminate forall (v:value) (fs_v:get_Type t) (tr':list event) (fs_tr':list fs_event). t ∋ ((fs_v, fs_tr'), (v, tr')) /\ (trace_related fs_tr' tr') ==> exists (tr'':list event) (fs_tr'':list fs_event).
-        qBool ⦂ ((ps' fs_v, fs_tr''), (subst_beta v (ELam?.b e_pt), tr'')) /\ (trace_related fs_tr'' tr'') /\ (tr_pt == tr' @ tr'') /\ (fs_tr == fs_tr' @ fs_tr'') 
-      with e_pt (backtranslate_ctx ct) [] [];
+    compile_equiv (dsnd ps);
+    let ps' = dfst ps in
+    compile_closed_equiv (dsnd ps);
+    assert ((t ^-> qBool) ⦂ (ps', pt));
+    lemma_compile_closed_arrow_is_elam (dsnd ps);
+    assert (ELam? pt /\ is_closed pt /\ irred pt);
+    eliminate forall (e':closed_exp). steps pt e' ==> irred e' ==> (t ^-> qBool) ∋ (ps', e') with pt;
+    assume ((t ^-> qBool) ∋ (ps', pt));
+    eliminate forall (v:value) (fs_v:get_Type t). t ∋ (fs_v, v) ==>
+        qBool ⦂ (ps' fs_v, subst_beta v (ELam?.b pt)) 
+      with e (backtranslate_ctx ct);
     lem_bt_ctx i ct;
-    assert (qBool ⦂ ((ps' (backtranslate_ctx ct), fs_tr), (subst_beta e (ELam?.b e_pt), tr_pt)));
-    lem_rel_beh (ps' (backtranslate_ctx ct)) fs_tr (subst_beta e (ELam?.b e_pt)) tr_pt;
-    assume (behT (EApp e_pt e) tr_pt == behT (subst_beta e (ELam?.b e_pt)) tr_pt); (** simple to prove **)
-    assume (tr_pt == tr_pt @ []);
+    assert (qBool ⦂ (ps' (backtranslate_ctx ct), subst_beta e (ELam?.b pt)));
+    lem_rel_beh (ps' (backtranslate_ctx ct)) (subst_beta e (ELam?.b pt));
+    assume (behT (EApp pt e) == behT (subst_beta e (ELam?.b pt))); (** simple to prove **)
     ()
   end
